Progress with properties of the "wave sort"

hol/wavefrontsScript.sml
@@ -1,7 +1,7 @@
 open HolKernel Parse boolLib bossLib;
 
 open actionGraphTheory datadepsTheory
-open sortingTheory relationTheory
+open pred_setTheory listTheory sortingTheory relationTheory
 
 open lcsymtacs
 
@@ -17,10 +17,102 @@ val transitive_LE = store_thm(
   "transitive_LE",
   ``transitive (<=)``,
   ASM_SIMP_TAC (srw_ss() ++ ARITH_ss) [transitive_def])
+val _ = export_rewrites ["transitive_LE"]
 
-val wavesort_def = Define`
-  wavesort G l =
-    QSORT (inv_image (inv_image (<=) (wave G) LEX (<=)) (λe. (e,e))) l
+val waveR_def = Define`
+  waveR G = inv_image (inv_image (<=) (wave G) LEX (<=)) (λe. (e,e))
 `;
+
+val GENLIST_EQ_NIL = store_thm(
+  "GENLIST_EQ_NIL",
+  ``(GENLIST f n = [] ⇔ n = 0) ∧
+    ([] = GENLIST f n ⇔ n = 0)``,
+  Cases_on `n` >> simp[GENLIST_CONS]);
+
+val GENLIST_EQ_CONS = store_thm(
+  "GENLIST_EQ_CONS",
+  ``GENLIST f n = h::t ⇔ ∃m. n = SUC m ∧ h = f 0 ∧ t = GENLIST (f o SUC) m``,
+  Cases_on `n` >> simp[GENLIST_CONS] >> metis_tac[]);
+
+val lift_splitAtPki_RAND = store_thm(
+  "lift_splitAtPki_RAND",
+  ``∀P k. f (splitAtPki P k l) = splitAtPki P ((o) f o k) l``,
+  Induct_on `l` >> simp[splitAtPki_DEF] >>
+  map_every qx_gen_tac [`h`, `P`, `k`] >>
+  Cases_on `P 0 h` >> simp[combinTheory.o_DEF]);
+
+val lift_splitAtPki_RATOR = store_thm(
+  "lift_splitAtPki_RATOR",
+  ``∀P k. splitAtPki P k l x =
+          splitAtPki P (combin$C (combin$C o k) x) l``,
+  Induct_on `l` >> simp[splitAtPki_DEF] >> rw[combinTheory.C_DEF]);
+
+val splitAtPki_l1 = prove(
+  ``splitAtPki P (λl1 l2. f l1) l = f (splitAtPki P (λl1 l2. l1) l)``,
+  CONV_TAC (RAND_CONV (REWR_CONV lift_splitAtPki_RAND)) >>
+  simp[combinTheory.o_DEF]);
+
+val findi_def = Define`
+  findi x [] = 0 ∧
+  findi x (h::t) = if x = h then 0 else 1 + findi x t
+`;
+
+val MEM_findi = prove(
+  ``MEM x l ⇒ findi x l < LENGTH l``,
+  Induct_on `l` >> simp[findi_def] >>
+  rw[arithmeticTheory.ADD1, arithmeticTheory.ZERO_LESS_ADD]);
+
+val BIJ_CONG = store_thm(
+  "BIJ_CONG",
+  ``s1 = s1' ⇒ s2 = s2' ⇒ (∀x. x ∈ s1' ⇒ f x = f' x) ⇒
+    (BIJ f s1 s2 ⇔ BIJ f' s1' s2')``,
+  SIMP_TAC (srw_ss() ++ boolSimps.CONJ_ss)
+           [BIJ_DEF, INJ_DEF, SURJ_DEF, EQ_IMP_THM]);
+
+val findi_EL = store_thm(
+  "findi_EL",
+  ``∀l n. n < LENGTH l ∧ ALL_DISTINCT l ⇒ findi (EL n l) l = n``,
+  Induct >> simp[] >> map_every qx_gen_tac [`h`, `n`] >> strip_tac >>
+  Cases_on `n` >> simp[findi_def] >> rw[arithmeticTheory.ADD1] >>
+  fs[] >> metis_tac[MEM_EL]);
+
+val PERM_BIJ = store_thm(
+  "PERM_BIJ",
+  ``∀l1 l2. PERM l1 l2 ⇒ ALL_DISTINCT l1 ⇒
+            BIJ (λx. EL (findi x l1) l2) (set l1) (set l1)``,
+  `∀x. PRE (x + 1) = x` by decide_tac >>
+  `∀x. PRE (x + 2) = x + 1` by decide_tac >>
+  Induct_on `PERM l1 l2` >> simp[BIJ_EMPTY] >> rpt strip_tac
+  >- (`∀y. y ∈ set l1 ⇒ y <> x` by metis_tac[] >>
+      simp[BIJ_INSERT, findi_def, DELETE_INSERT, DELETE_NON_ELEMENT_RWT,
+           Cong BIJ_CONG, rich_listTheory.EL_CONS])
+  >- (`∀z. z ∈ set l1 ⇒ z <> x ∧ z <> y` by metis_tac[] >>
+      simp[BIJ_INSERT, findi_def, DELETE_INSERT, DELETE_NON_ELEMENT_RWT,
+           Cong BIJ_CONG, rich_listTheory.EL_CONS]) >>
+  `ALL_DISTINCT l1'` by metis_tac [ALL_DISTINCT_PERM] >> fs[] >>
+  `set l1' = set l1 ∧ LENGTH l1' = LENGTH l1`
+    by metis_tac [PERM_LIST_TO_SET, PERM_LENGTH] >> fs[] >>
+  `∀x. x ∈ set l1 ⇒
+       EL (findi (EL (findi x l1) l1') l1') l2 = EL (findi x l1) l2`
+    by simp[findi_EL, MEM_findi] >>
+  `BIJ ((λx. EL (findi x l1') l2) o (λx. EL (findi x l1) l1'))
+       (set l1) (set l1)`
+    by metis_tac [BIJ_COMPOSE] >>
+  pop_assum mp_tac >> simp[Cong BIJ_CONG])
+
+val wavesort_sorted = store_thm(
+  "wavesort_sorted",
+  ``SORTED (waveR G) (QSORT (waveR G) l)``,
+  match_mp_tac QSORT_SORTED >> simp[waveR_def]);
+
+(*
+val SORTED_SEPARATED_ELEMENTS = store_thm(
+  "SORTED_SEPARATED_ELEMENTS",
+  ``transitive R ∧ SORTED R l ⇒
+    ∀i j. i < j ∧ j < LENGTH l ⇒ R (EL i l) (EL j l)``,
+  Induct_on `l` >> simp[] >> qx_gen_tac `h` >>
+  Cases_on `l` >> simp[SORTED_DEF]
+*)
+
 
 val _ = export_theory();
